aarch64 infoflow: prove noninterference
Signed-off-by: Ryan Barry <ryan.barry@proofcraft.systems>

proof/infoflow/AARCH64/ArchFinalise_IF.thy
@@ -8,7 +8,7 @@ theory ArchFinalise_IF
 imports Finalise_IF
 begin
 
-context Arch begin global_naming AARCH64
+context Arch begin arch_global_naming
 
 named_theorems Finalise_IF_assms
 
@@ -18,14 +18,7 @@ crunch arch_post_cap_deletion
 
 lemma dmo_maskInterrupt_reads_respects[Finalise_IF_assms]:
   "reads_respects aag l \<top> (do_machine_op (maskInterrupt m irq))"
-  unfolding maskInterrupt_def
-  apply (rule use_spec_ev)
-  apply (rule do_machine_op_spec_reads_respects)
-   apply (simp add: equiv_valid_def2)
-   apply (rule modify_ev2)
-   apply (fastforce simp: equiv_for_def)
-  apply (wp modify_wp | simp)+
-  done
+  by wpsimp
 
 lemma arch_post_cap_deletion_read_respects[Finalise_IF_assms, wp]:
   "reads_respects aag l \<top> (arch_post_cap_deletion acap)"
@@ -69,8 +62,8 @@ lemma set_thread_state_reads_respects[Finalise_IF_assms]:
      apply (rule set_thread_state_act_reads_respects)
     apply (case_tac "aag_can_read aag ref \<or> aag_can_affect aag l ref")
      apply (wp set_object_reads_respects gets_the_ev)
-     apply (fastforce simp: get_tcb_def split: option.splits
-                     elim: reads_equivE affects_equivE equiv_forE)
+     apply fastforce
+    apply (clarsimp simp: equiv_for_def get_tcb_def)
     apply (simp add: equiv_valid_def2)
     apply (rule equiv_valid_rv_bind)
       apply (rule equiv_valid_rv_trivial)
@@ -96,7 +89,8 @@ lemma set_thread_state_runnable_reads_respects[Finalise_IF_assms]:
      apply (rule set_thread_state_act_runnable_reads_respects)
     apply (case_tac "aag_can_read aag ref \<or> aag_can_affect aag l ref")
      apply (wp set_object_reads_respects gets_the_ev)
-     apply (fastforce simp: get_tcb_def split: option.splits elim: reads_equivE affects_equivE equiv_forE)
+     apply fastforce
+    apply (clarsimp simp: equiv_for_def get_tcb_def)
     apply (simp add: equiv_valid_def2)
     apply (rule equiv_valid_rv_bind)
       apply (rule equiv_valid_rv_trivial)
@@ -110,7 +104,7 @@ lemma set_thread_state_runnable_reads_respects[Finalise_IF_assms]:
     apply (blast dest: get_tcb_not_asid_pool_at)
    apply (subst thread_set_def[symmetric, simplified fun_app_def])
    apply (wp thread_set_st_tcb_at | simp)+
-   done
+  done
 
 lemma set_bound_notification_none_reads_respects[Finalise_IF_assms]:
   assumes domains_distinct: "pas_domains_distinct aag"
@@ -119,7 +113,8 @@ lemma set_bound_notification_none_reads_respects[Finalise_IF_assms]:
   apply (rule pre_ev(5)[where Q=\<top>])
    apply (case_tac "aag_can_read aag ref \<or> aag_can_affect aag l ref")
     apply (wp set_object_reads_respects gets_the_ev)[1]
-    apply (fastforce simp: get_tcb_def split: option.splits elim: reads_equivE affects_equivE equiv_forE)
+    apply fastforce
+   apply (clarsimp simp: equiv_for_def get_tcb_def)
    apply (simp add: equiv_valid_def2)
    apply (rule equiv_valid_rv_bind)
      apply (rule equiv_valid_rv_trivial)
@@ -152,7 +147,8 @@ lemma set_tcb_queue_modifies_at_most:
   "modifies_at_most aag L (\<lambda>s. pasDomainAbs aag d \<inter> L \<noteq> {}) (set_tcb_queue d prio queue)"
   apply (rule modifies_at_mostI)
   apply (simp add: set_tcb_queue_def modify_def, wp)
-  apply (force simp: equiv_but_for_labels_def states_equiv_for_def equiv_for_def equiv_asids_def)
+  apply (force simp: equiv_but_for_labels_def states_equiv_for_def equiv_for_def equiv_asids_def
+                     equiv_hyp_def equiv_fpu_def cur_fpu_for_def get_tcb_def)
   done
 
 lemma set_notification_equiv_but_for_labels[Finalise_IF_assms]:
@@ -165,21 +161,16 @@ lemma set_notification_equiv_but_for_labels[Finalise_IF_assms]:
   done
 
 lemma thread_set_reads_respects[Finalise_IF_assms]:
-  assumes domains_distinct[wp]: "pas_domains_distinct aag"
-  shows "reads_respects aag l \<top> (thread_set x y)"
-  unfolding thread_set_def fun_app_def
-  apply (case_tac "aag_can_read aag y \<or> aag_can_affect aag l y")
-   apply (wp set_object_reads_respects)
-   apply (clarsimp, rule reads_affects_equiv_get_tcb_eq, simp+)[1]
-  apply (simp add: equiv_valid_def2)
-  apply (rule equiv_valid_rv_guard_imp)
-   apply (rule_tac L="{pasObjectAbs aag y}" and L'="{pasObjectAbs aag y}"
-                in ev2_invisible[OF domains_distinct])
-       apply (assumption | simp add: labels_are_invisible_def)+
-     apply (rule modifies_at_mostI[where P="\<top>"]
-            | wp set_object_equiv_but_for_labels
-            | simp
-            | (clarify, drule get_tcb_not_asid_pool_at))+
+  "reads_respects aag l \<top> (thread_set f thread)"
+  apply (rule equiv_valid_guard_imp)
+   apply (rule_tac ptr=thread in reads_respects_unit_cases)
+  unfolding thread_set_def
+     apply (rule gen_asm_ev)
+     apply (wpsimp wp: set_object_reads_respects)
+    apply (wpsimp wp: set_object_equiv_but_for_labels)
+    apply (clarsimp simp: get_tcb_def obj_at_def)
+   apply wpsimp+
+  apply auto
   done
 
 lemma aag_cap_auth_ASIDPoolCap:
@@ -190,7 +181,7 @@ lemma aag_cap_auth_ASIDPoolCap:
                 cli_no_irqs pas_refined_all_auth_is_owns)
 
 lemma aag_cap_auth_PageDirectory:
-  "pas_cap_cur_auth aag (ArchObjectCap (PageTableCap word (Some a))) \<Longrightarrow>
+  "pas_cap_cur_auth aag (ArchObjectCap (PageTableCap word pt_t (Some a))) \<Longrightarrow>
     pas_refined aag s \<Longrightarrow> is_subject aag word"
   unfolding aag_cap_auth_def
   by (simp add: clas_no_asid cap_auth_conferred_def arch_cap_auth_conferred_def
@@ -213,27 +204,27 @@ lemma aag_cap_auth_PageCap_asid:
           intro: pas_refined_Control_into_is_subject_asid)
 
 lemma aag_cap_auth_PageTableCap:
-  "\<lbrakk> pas_cap_cur_auth aag (ArchObjectCap (PageTableCap word option)); pas_refined aag s \<rbrakk>
+  "\<lbrakk> pas_cap_cur_auth aag (ArchObjectCap (PageTableCap word pt_t option)); pas_refined aag s \<rbrakk>
      \<Longrightarrow> is_subject aag word"
   unfolding aag_cap_auth_def
   by (simp add: clas_no_asid cap_auth_conferred_def arch_cap_auth_conferred_def
                 cli_no_irqs pas_refined_all_auth_is_owns)
 
 lemma aag_cap_auth_PageTableCap_asid:
-  "\<lbrakk> pas_cap_cur_auth aag (ArchObjectCap (PageTableCap word (Some (a, b)))); pas_refined aag s \<rbrakk>
+  "\<lbrakk> pas_cap_cur_auth aag (ArchObjectCap (PageTableCap word pt_t (Some (a, b)))); pas_refined aag s \<rbrakk>
      \<Longrightarrow> is_subject_asid aag a"
   by (auto simp: aag_cap_auth_def cap_links_asid_slot_def label_owns_asid_slot_def
           intro: pas_refined_Control_into_is_subject_asid)
 
 lemma aag_cap_auth_PageDirectoryCap:
-  "\<lbrakk> pas_cap_cur_auth aag (ArchObjectCap (PageTableCap word option));  pas_refined aag s \<rbrakk>
+  "\<lbrakk> pas_cap_cur_auth aag (ArchObjectCap (PageTableCap word pt_t option));  pas_refined aag s \<rbrakk>
      \<Longrightarrow> is_subject aag word"
   unfolding aag_cap_auth_def
   by (simp add: clas_no_asid cap_auth_conferred_def arch_cap_auth_conferred_def
                 cli_no_irqs pas_refined_all_auth_is_owns)
 
 lemma aag_cap_auth_PageDirectoryCap_asid:
-  "\<lbrakk> pas_cap_cur_auth aag (ArchObjectCap (PageTableCap word (Some (a,vref)))); pas_refined aag s \<rbrakk>
+  "\<lbrakk> pas_cap_cur_auth aag (ArchObjectCap (PageTableCap word pt_t (Some (a,vref)))); pas_refined aag s \<rbrakk>
      \<Longrightarrow> is_subject_asid aag a"
   unfolding aag_cap_auth_def
   by (auto simp: cap_links_asid_slot_def label_owns_asid_slot_def
@@ -243,11 +234,737 @@ lemmas aag_cap_auth_subject = aag_cap_auth_ASIDPoolCap_asid
                               aag_cap_auth_PageCap_asid
                               aag_cap_auth_PageTableCap_asid
 
+(* Helpful groupings *)
+
+definition fpu_save where
+  "fpu_save \<equiv> do
+     cur_fpu_owner \<leftarrow> gets (arm_current_fpu_owner \<circ> arch_state);
+     do_machine_op enableFpu;
+     maybeM save_fpu_state cur_fpu_owner
+  od"
+
+definition fpu_restore where
+  "fpu_restore new_owner \<equiv> do
+     case new_owner of None \<Rightarrow> do_machine_op disableFpu
+        | Some tcb_ptr \<Rightarrow> load_fpu_state tcb_ptr;
+     set_arm_current_fpu_owner new_owner
+   od"
+
+lemma dmo_enableFpu_reads_respects[wp]:
+  "states_equiv_valid aag L \<top> (do_machine_op enableFpu)"
+  unfolding enableFpu_def dmo_distr
+  apply wpsimp
+     apply (wpsimp wp: do_machine_op_states_equiv_valid modify_ev)
+       apply (clarsimp simp: equiv_for_def)
+      apply (wpsimp wp: dmo_mol_states_equiv_valid)+
+  done
+
+lemma dmo_disableFpu_states_equiv_valid[wp]:
+  "states_equiv_valid aag L \<top> (do_machine_op disableFpu)"
+  unfolding disableFpu_def dmo_distr
+  apply wpsimp
+     apply (wpsimp wp: do_machine_op_states_equiv_valid modify_ev)
+       apply (clarsimp simp: equiv_for_def)
+      apply (wpsimp wp: dmo_mol_states_equiv_valid)+
+  done
+
+lemma switch_local_fpu_owner_def2:
+  "switch_local_fpu_owner new_owner = do fpu_save; fpu_restore new_owner od"
+  unfolding switch_local_fpu_owner_def fpu_save_def fpu_restore_def
+  by (clarsimp simp: bind_assoc)
+
+lemma valid_cur_fpu_cur_fpu_for:
+  "valid_cur_fpu s \<Longrightarrow> cur_fpu_for P s = (\<exists>p. P p \<and> is_tcb_cur_fpu p s)"
+  apply (clarsimp simp: cur_fpu_for_def valid_cur_fpu_def)
+  apply (rule iffI; erule ex_forward)
+   apply (clarsimp simp: valid_cur_fpu_def is_tcb_cur_fpu_def obj_at_def get_tcb_def is_arch_cur_fpu_def
+                  split: option.splits kernel_object.splits)+
+  done
+
+lemma equiv_kheap_equiv_current_fpu:
+  "\<lbrakk> equiv_for P kheap s t; valid_cur_fpu s; valid_cur_fpu t; cur_fpu_for P s; cur_fpu_for P t\<rbrakk>
+     \<Longrightarrow> current_fpu s = current_fpu t"
+  apply (clarsimp simp: valid_cur_fpu_cur_fpu_for valid_cur_fpu_def
+                        equiv_for_def is_tcb_cur_fpu_def obj_at_def)
+  apply (drule_tac x=p in spec)+
+  apply auto
+  done
+
+(* FIXME AARCH64 IF: move *)
+lemma maybeM_when:
+  "maybeM f opt = when (opt \<noteq> None) (f (the opt))"
+  by (clarsimp simp: maybeM_def when_def)
+
+lemma maybeM_ev:
+  "\<lbrakk> \<And>v. opt = Some v \<Longrightarrow> equiv_valid_inv I A (P v) (f v) \<rbrakk>
+     \<Longrightarrow> equiv_valid_inv I A (\<lambda>s. \<forall>v. opt = Some v \<longrightarrow> P v s) (maybeM f opt)"
+  apply (subst maybeM_when)
+  apply (rule equiv_valid_guard_imp)
+   apply (rule_tac P="P (the opt)" in when_ev)
+   apply auto
+  done
+
+lemma as_user_states_equiv_valid_roa:
+  "states_equiv_valid aag L (K (det f \<and> (L (pasObjectAbs aag thread)))) (as_user thread f)"
+  apply (simp add: as_user_def split_def)
+  apply (rule gen_asm_ev)
+  apply (wp set_object_states_equiv_valid select_f_ev gets_the_ev)
+  apply (auto simp: equiv_for_def get_tcb_def arch_tcb_context_set_def states_equiv_for_def)
+  done
+
+lemma states_equiv_valid_unobservable_unit_return:
+  assumes f:
+    "\<And>P Q R S st. \<lbrace>states_equiv_for P Q R S st\<rbrace> f \<lbrace>\<lambda>_. states_equiv_for P Q R S st\<rbrace>"
+  shows
+    "states_equiv_valid aag L \<top> (f::(unit,det_ext) s_monad)"
+  apply (clarsimp simp: equiv_valid_def2 equiv_valid_2_def)
+  apply (erule use_valid[OF _ f])
+  apply (rule states_equiv_for_sym)
+  apply (erule use_valid[OF _ f])
+  apply (rule states_equiv_for_sym)
+  apply simp
+  done
+
+lemma dmo_readFpuState_states_equiv_valid:
+  "states_equiv_valid aag L (cur_fpu_for (L o pasObjectAbs aag)) (do_machine_op readFpuState)"
+  (is "states_equiv_valid _ _ ?P _")
+  unfolding readFpuState_def dmo_distr
+  apply (rule_tac Q="\<lambda>_. ?P" in bind_ev_pre)
+     apply wpsimp
+     apply (rule do_machine_op_states_equiv_valid')
+      apply (wpsimp wp: gets_ev')
+     apply (clarsimp simp: pred_disj_def equiv_fpu_state_def hw_fpu_def)
+    apply (rule states_equiv_valid_unobservable_unit_return)
+    apply (wpsimp wp: dmo_wp)+
+  done
+
+lemma det_setFPUStat[simp]:
+  "det (setFPUState fpu)"
+  by (wpsimp simp: setFPUState_def)
+
+lemma thread_set_equiv_but_for_labels[wp]:
+  "\<lbrace>equiv_but_for_labels aag L st and K (pasObjectAbs aag ptr \<in> L)\<rbrace>
+   thread_set f ptr
+   \<lbrace>\<lambda>_. equiv_but_for_labels aag L st\<rbrace>"
+  unfolding thread_set_def
+  apply (wpsimp wp: set_object_equiv_but_for_labels)
+  apply (clarsimp simp: get_tcb_def obj_at_def split: option.splits kernel_object.splits)
+  done
+
+lemma as_user_equiv_but_for_labels[wp]:
+  "\<lbrace>equiv_but_for_labels aag L st and K (pasObjectAbs aag ptr \<in> L)\<rbrace>
+   as_user ptr f
+   \<lbrace>\<lambda>_. equiv_but_for_labels aag L st\<rbrace>"
+  by (wpsimp wp: as_user_wp_thread_set_helper)
+
+lemma dmo_readFpuState_inv[wp]:
+  "do_machine_op readFpuState \<lbrace>P\<rbrace>"
+  by (wpsimp simp: readFpuState_def wp: dmo_wp)
+
+lemma save_fpu_state_states_equiv_valid:
+  "states_equiv_valid aag L (\<lambda>s. current_fpu s = Some ptr) (save_fpu_state ptr)"
+  (is "states_equiv_valid _ _ ?P _")
+  unfolding save_fpu_state_def
+  apply (rule equiv_valid_guard_imp)
+   apply (rule_tac P="?P" and ptr=ptr in states_equiv_valid_unit_cases)
+     apply (wpsimp wp: as_user_states_equiv_valid_roa dmo_readFpuState_states_equiv_valid)
+     apply (clarsimp simp: cur_fpu_for_def is_arch_cur_fpu_def)
+    apply wpsimp+
+  done
+
+(* FIXME AARCH64 IF: move *)
+locale_abbrev "cur_fpu_of s \<equiv> \<lambda>x. arm_current_fpu_owner (arch_state s) = Some x"
+
+lemma equiv_fpu_def2:
+  "equiv_fpu P s s' \<equiv> (\<forall>x. P x \<longrightarrow>
+     (current_fpu s = Some x \<longleftrightarrow> current_fpu s' = Some x) \<and>
+     (current_fpu s = Some x \<longrightarrow> machine_fpu s = machine_fpu s'))"
+  apply (rule eq_reflection)
+  apply (clarsimp simp: equiv_fpu_def equiv_for_def valid_cur_fpu_cur_fpu_for)
+  apply (clarsimp simp: hw_fpu_def is_arch_cur_fpu_def)
+  apply auto
+  done
+
+lemma dmo_disableFpu_machine_fpu[wp]:
+  "do_machine_op disableFpu \<lbrace>\<lambda>s. P (machine_fpu s)\<rbrace>"
+  by (wpsimp wp: dmo_wp)
+
+lemma dmo_enableFpu_machine_fpu[wp]:
+  "do_machine_op enableFpu \<lbrace>\<lambda>s. P (machine_fpu s)\<rbrace>"
+  by (wpsimp wp: dmo_wp)
+
+lemma tcb_at_typ_at':
+  "(\<And>P T p. \<lbrace>\<lambda>s. P (typ_at T p s)\<rbrace> f \<lbrace>\<lambda>rv s. P (typ_at T p s)\<rbrace>)
+   \<Longrightarrow> \<lbrace>\<lambda>s. P (tcb_at c s)\<rbrace> f \<lbrace>\<lambda>rv s. P (tcb_at c s)\<rbrace>"
+  by (simp add: tcb_at_typ)
+
+lemma as_user_not_tcb_at[wp]:
+  "as_user t m \<lbrace>\<lambda>s. \<not>tcb_at t' s\<rbrace>"
+  by (wpsimp wp: tcb_at_typ_at'[OF as_user_typ_at])
+
+crunch save_fpu_state
+  for not_tcb_at[wp]: "\<lambda>s. \<not>tcb_at t s"
+
+lemma fpu_of_Some_True[simp]:
+  "fpu_of (Some True) fopt fpu = Some fpu"
+  by (clarsimp simp: fpu_of_def)
+
+lemma fpu_of_Some_False[simp]:
+  "fpu_of (Some False) fopt fpu = fopt"
+  by (clarsimp simp: fpu_of_def)
+
+lemma fpu_of_None[simp]:
+  "fpu_of None fopt fpu = None"
+  by (clarsimp simp: fpu_of_def)
+
+lemma valid_cur_fpu_current_fpu_Some:
+  "\<lbrakk> valid_cur_fpu s; current_fpu s = Some t \<rbrakk>
+     \<Longrightarrow> tcb_cur_fpu_of s t = Some True"
+  apply (clarsimp simp: valid_cur_fpu_def)
+  apply (erule_tac x=t in allE)
+  apply (clarsimp simp: get_tcb_def is_tcb_cur_fpu_def obj_at_def)
+  done
+
+lemma save_fpu_state_equiv_but_for_labels[wp]:
+  "\<lbrace>\<lambda>s. equiv_but_for_labels aag L st s \<and> pasObjectAbs aag ptr \<in> L\<rbrace>
+   save_fpu_state ptr
+   \<lbrace>\<lambda>_. equiv_but_for_labels aag L st\<rbrace>"
+  unfolding save_fpu_state_def
+  by wpsimp
+
+lemma dmo_enableFpu_equiv_but_for_labels[wp]:
+  "do_machine_op enableFpu \<lbrace>equiv_but_for_labels aag L st\<rbrace>"
+  by (wpsimp wp: dmo_equiv_but_for_labels_lift)
+
+lemma dmo_disableFpu_equiv_but_for_labels[wp]:
+  "do_machine_op disableFpu \<lbrace>equiv_but_for_labels aag L st\<rbrace>"
+  by (wpsimp wp: dmo_equiv_but_for_labels_lift)
+
+lemma fpu_save_states_equiv_valid:
+  "states_equiv_valid aag L valid_cur_fpu fpu_save"
+  unfolding fpu_save_def
+  apply (rule_tac P="cur_fpu_for (L o pasObjectAbs aag)" in equiv_valid_cases'')
+    apply (fastforce simp: states_equiv_for_def comp_def equiv_fpu_cur_fpu_for)
+   apply (wpsimp wp: maybeM_ev gets_ev'' save_fpu_state_states_equiv_valid
+                     hoare_vcg_imp_lift' hoare_vcg_all_lift)
+     apply (rename_tac s t)
+     apply (prop_tac "valid_cur_fpu s \<and> cur_fpu_for (L o pasObjectAbs aag) s")
+      apply assumption
+     apply (prop_tac "valid_cur_fpu t \<and> cur_fpu_for (L o pasObjectAbs aag) t")
+      apply assumption
+     apply clarsimp
+     apply (prop_tac "equiv_for (L o pasObjectAbs aag) kheap s t")
+      apply (fastforce simp: states_equiv_for_def comp_def)
+     apply (clarsimp simp: equiv_kheap_equiv_current_fpu)
+    apply wpsimp
+   apply clarsimp
+  apply (rule wp_pre)
+   apply (simp add: equiv_valid_def2)
+   apply (rule_tac R'="\<top>\<top>"
+               and Q="\<lambda>rv. (\<lambda>s. current_fpu s = rv \<and> valid_cur_fpu s)
+                           and K (\<forall>vr. rv = Some vr \<longrightarrow> \<not> L (pasObjectAbs aag vr))"
+               and Q'="\<lambda>rv. (\<lambda>s. current_fpu s = rv \<and> valid_cur_fpu s)
+                            and K (\<forall>vr. rv = Some vr \<longrightarrow> \<not> L (pasObjectAbs aag vr))"
+                in equiv_valid_2_bind)
+      apply (rule EquivValid.gen_asm_ev2_l)
+      apply (rule EquivValid.gen_asm_ev2_r)
+      prefer 2
+      apply (rule gets_any_evrv)
+     apply (rule equiv_valid_2_guard_imp)
+       apply (rule states_equiv_valid_2_invisible)
+           apply (rule modifies_at_mostI)
+           apply (wpsimp wp: hoare_vcg_imp_lift hoare_vcg_all_lift)
+          apply (rule modifies_at_mostI)
+          apply (wpsimp wp: hoare_vcg_imp_lift hoare_vcg_all_lift)
+         apply (wp | simp)+
+  apply (auto simp: cur_fpu_for_def is_arch_cur_fpu_def)
+  done
+
+lemma equiv_valid_lift:
+  assumes "\<And>P. f \<lbrace>\<lambda>s. P (i s)\<rbrace>"
+  shows "equiv_valid (equiv_for P i) \<top>\<top> \<top>\<top> \<top> (f :: ('s state, unit) nondet_monad)"
+  apply (clarsimp simp: equiv_valid_def2 equiv_valid_2_def)
+  apply (erule use_valid)
+   apply (wpsimp wp: assms equiv_for_lift)
+  apply (erule use_valid)
+   apply (wpsimp wp: assms equiv_for_lift)
+  apply clarsimp
+  done
+
+crunch getFPUState
+  for inv[wp]: P
+
+crunch load_fpu_state
+  for kheap[wp]: "\<lambda>s. P (kheap s)"
+  (wp: as_user_inv)
+
+lemma set_object_equiv_kheap:
+  "equiv_valid_inv (equiv_for P kheap) \<top>\<top> \<top> (set_object ptr obj)"
+  by (clarsimp simp: equiv_valid_def2 equiv_valid_2_def set_object_def get_object_def
+                     bind_def' get_def gets_def put_def return_def fail_def assert_def equiv_for_def)
+
+lemma thread_set_kheap_equiv:
+  "equiv_valid_inv (equiv_for P kheap) \<top>\<top> \<top> (thread_set f thread)"
+  unfolding thread_set_def
+  apply (case_tac "P thread")
+   apply (wpsimp wp: set_object_equiv_kheap)
+   apply (clarsimp simp: get_tcb_def equiv_for_def)
+  apply (clarsimp simp: equiv_valid_def2 equiv_valid_2_def set_object_def get_object_def
+                        gets_the_def assert_opt_def get_tcb_def bind_def' get_def gets_def
+                        put_def return_def fail_def assert_def equiv_for_def
+                 split: option.splits kernel_object.splits)
+  done
+
+lemma arch_thread_set_kheap_equiv:
+  "equiv_valid_inv (equiv_for P kheap) \<top>\<top> \<top> (arch_thread_set f thread)"
+  by (wpsimp simp: arch_thread_set_is_thread_set wp: thread_set_kheap_equiv)
+
+lemma gets_current_fpu_owner_equiv_kheap:
+  "equiv_valid (equiv_for P kheap) (equiv_for P cur_fpu_of) (\<lambda>_ _. True)
+               (valid_cur_fpu and cur_fpu_for P)
+               (gets (arm_current_fpu_owner \<circ> arch_state))"
+  (is "equiv_valid_inv _ _ ?P _")
+  apply (clarsimp simp: equiv_valid_def2 equiv_valid_2_def gets_def get_def return_def bind_def)
+  apply (clarsimp simp: equiv_for_def cur_fpu_for_def is_arch_cur_fpu_def)
+  done
+
+lemma equiv_valid_make_inv:
+  assumes "equiv_valid_inv I A P f"
+  shows "equiv_valid I A \<top>\<top> P f"
+  using assms
+  by (fastforce simp: equiv_valid_def2 equiv_valid_2_def)
+
+lemma arch_thread_set_equiv_for_kheap:
+  "\<lbrace>equiv_for P kheap st and K (\<not>P thread)\<rbrace>
+   arch_thread_set f thread
+   \<lbrace>\<lambda>_. equiv_for P kheap st\<rbrace>"
+  apply (wpsimp wp: arch_thread_set_wp)
+  apply (clarsimp simp: equiv_for_def)
+  done
+
+lemma set_arm_current_fpu_owner_ev:
+  "equiv_valid (equiv_for P kheap) (equiv_for P cur_fpu_of) \<top>\<top> (valid_cur_fpu)
+    (do cur_fpu_owner <- gets (arm_current_fpu_owner \<circ> arch_state);
+        maybeM (arch_thread_set (tcb_cur_fpu_update (\<lambda>_. False))) cur_fpu_owner
+     od)"
+  apply (rule_tac P="cur_fpu_for P" in equiv_valid_cases'')
+    apply (fastforce simp: equiv_for_def cur_fpu_for_def is_arch_cur_fpu_def)
+   apply (rule wp_pre)
+    apply (rule bind_ev_general)
+      apply (wp maybeM_ev)
+      apply (wpsimp wp: maybeM_ev arch_thread_set_kheap_equiv)
+     apply (wp gets_current_fpu_owner_equiv_kheap)
+    apply wpsimp
+   apply clarsimp
+  apply (rule equiv_valid_make_inv)
+  apply (rule equiv_valid_inv_lift)
+    apply (wpsimp wp: arch_thread_set_equiv_for_kheap equiv_for_lift)
+    apply (clarsimp simp: equiv_for_def cur_fpu_for_def is_arch_cur_fpu_def)
+   apply (auto simp: equiv_for_sym)
+  done
+
+crunch load_fpu_state
+  for valid_cur_fpu[wp]: valid_cur_fpu
+
+lemma fpu_restore_equiv_kheap':
+  "equiv_valid (equiv_for P kheap) (equiv_for P cur_fpu_of) \<top>\<top> valid_cur_fpu (fpu_restore new_owner)"
+  unfolding fpu_restore_def set_arm_current_fpu_owner_def
+  apply (rule equiv_valid_guard_imp)
+   apply (rule_tac A=B and B=B for B in bind_ev_general)
+     prefer 2
+     apply (rule equiv_valid_inv_lift)
+       apply (wpsimp wp: equiv_for_lift)+
+      apply (fastforce simp: equiv_for_def)+
+    apply simp
+    apply (subst bind_assoc[symmetric])
+    apply (rule bind_ev_general)
+      prefer 2
+      apply (rule set_arm_current_fpu_owner_ev)
+     apply clarsimp
+     apply (rule bind_ev_general)
+       prefer 2
+       apply (rule equiv_valid_lift)
+       apply wpsimp
+      apply (rule maybeM_ev)
+      apply (rule arch_thread_set_kheap_equiv)
+     apply wpsimp+
+  done
+
+lemma fpu_restore_equiv_kheap:
+  "equiv_valid (equiv_for P kheap) (equiv_fpu P) \<top>\<top> valid_cur_fpu (fpu_restore new_owner)"
+  apply (rule equiv_valid_conseq)
+    apply (rule_tac P=P in fpu_restore_equiv_kheap')
+   apply (clarsimp simp: equiv_fpu_def2 equiv_for_def)
+  apply clarsimp
+  done
+
+crunch fpu_save
+  for valid_cur_fpu[wp]: "valid_cur_fpu"
+  (wp: crunch_wps)
+
+lemma switch_local_fpu_owner_equiv_kheap:
+  "equiv_valid \<top>\<top> (states_equiv_for_labels aag L) (equiv_for (L o pasObjectAbs aag) kheap)
+               valid_cur_fpu (switch_local_fpu_owner new_owner :: (det_state,unit) nondet_monad)"
+  unfolding switch_local_fpu_owner_def2
+  apply (rule equiv_valid_guard_imp)
+   apply (rule_tac B="\<lambda>s t. equiv_for (L \<circ> pasObjectAbs aag) kheap s t \<and>
+                            equiv_fpu (L \<circ> pasObjectAbs aag) s t"
+               and P'=valid_cur_fpu in bind_ev_general)
+  by (wpsimp wp: fpu_restore_equiv_kheap[where P="L o pasObjectAbs aag"]
+                 fpu_save_states_equiv_valid[where aag=aag and L=L]
+           simp: comp_def states_equiv_for_def equiv_for_disj equiv_fpu_def
+      | rule equiv_valid_conseq[where P=valid_cur_fpu] | fastforce)+
+
+definition states_equiv_for_non_fpu ::
+  "(obj_ref \<Rightarrow> bool) \<Rightarrow> (irq \<Rightarrow> bool) \<Rightarrow> (asid \<Rightarrow> bool) \<Rightarrow>
+   (domain \<Rightarrow> bool) \<Rightarrow> det_state \<Rightarrow> det_state \<Rightarrow> bool" where
+  "states_equiv_for_non_fpu P Q R S s s' \<equiv>
+     equiv_machine_state P (machine_state s) (machine_state s') \<and>
+     equiv_for (P \<circ> fst) cdt s s' \<and>
+     equiv_for (P \<circ> fst) cdt_list s s' \<and>
+     equiv_for (P \<circ> fst) is_original_cap s s' \<and>
+     equiv_for Q interrupt_states s s' \<and>
+     equiv_for Q interrupt_irq_node s s' \<and>
+     equiv_for S ready_queues s s' \<and>
+     equiv_asids R s s' \<and>
+     equiv_hyp P s s'"
+
+lemma states_equiv_for_non_fpu_refl:
+  "states_equiv_for_non_fpu P Q R S s s"
+  by (auto simp: states_equiv_for_non_fpu_def intro: equiv_for_refl equiv_asids_refl equiv_hyp_refl)
+
+lemma states_equiv_for_non_fpu_sym:
+  "states_equiv_for_non_fpu P Q R S s t \<Longrightarrow> states_equiv_for_non_fpu P Q R S t s"
+  by (auto simp: states_equiv_for_non_fpu_def intro: equiv_for_sym equiv_asids_sym equiv_fpu_sym equiv_hyp_sym)
+
+lemma states_equiv_for_non_fpu_trans:
+  "\<lbrakk> states_equiv_for_non_fpu P Q R S s t; states_equiv_for_non_fpu P Q R S t u \<rbrakk>
+     \<Longrightarrow> states_equiv_for_non_fpu P Q R S s u"
+  by (auto simp: states_equiv_for_non_fpu_def
+          intro: equiv_for_trans equiv_asids_trans equiv_fpu_trans equiv_hyp_trans equiv_forI
+           elim: equiv_forE)
+
+abbreviation states_equiv_for_labels_non_fpu ::
+  "'a PAS \<Rightarrow> ('a \<Rightarrow> bool) \<Rightarrow> det_state \<Rightarrow> det_state \<Rightarrow> bool" where
+  "states_equiv_for_labels_non_fpu aag P \<equiv>
+      states_equiv_for_non_fpu (\<lambda>x. P (pasObjectAbs aag x)) (\<lambda>x. P (pasIRQAbs aag x))
+                               (\<lambda>x. P (pasASIDAbs aag x)) (\<lambda>x. \<exists>l\<in>pasDomainAbs aag x. P l)"
+
+abbreviation states_equiv_valid_non_fpu where
+  "states_equiv_valid_non_fpu aag L P f \<equiv> equiv_valid_inv \<top>\<top> (states_equiv_for_labels_non_fpu aag L) P f"
+
+lemma states_equiv_for_non_fpu_symmetric:
+  "states_equiv_for_non_fpu P Q R S s t \<Longrightarrow> states_equiv_for_non_fpu P Q R S t s"
+  by (auto simp: states_equiv_for_non_fpu_sym)
+
+lemma states_equiv_valid_non_fpu_unobservable:
+  assumes "\<And>P Q R S st. f \<lbrace>states_equiv_for_non_fpu P Q R S st\<rbrace>"
+  assumes "\<And>P. f \<lbrace>\<lambda>s. P (cur_thread s)\<rbrace>"
+  assumes "\<And>P. f \<lbrace>\<lambda>s. P (cur_domain s)\<rbrace>"
+  assumes "\<And>P. f \<lbrace>\<lambda>s. P (scheduler_action s)\<rbrace>"
+  assumes "\<And>P. f \<lbrace>\<lambda>s. P (work_units_completed s)\<rbrace>"
+  assumes l: "\<And>P. f \<lbrace>\<lambda>s. P (irq_state (machine_state s))\<rbrace>"
+  shows "states_equiv_valid_non_fpu aag l \<top> (f :: (det_state,unit) nondet_monad)"
+  apply (clarsimp simp: equiv_valid_def2 equiv_valid_2_def)
+  apply (rule states_equiv_for_non_fpu_symmetric)
+  apply (erule use_valid)
+   apply (wp assms)
+  apply (rule states_equiv_for_non_fpu_symmetric)
+  apply (erule use_valid)
+   apply (wp assms)
+  apply simp
+  done
+
+lemma equiv_hyp_lift:
+  assumes "\<And>P. f \<lbrace>\<lambda>s. P (vcpu_state (machine_state s))\<rbrace>"
+  assumes "\<And>P. f \<lbrace>\<lambda>s. P (current_vcpu s)\<rbrace>"
+  assumes "\<And>P. f \<lbrace>\<lambda>s. P (numlistregs s)\<rbrace>"
+  shows "f \<lbrace>\<lambda>s. equiv_hyp P st s\<rbrace>"
+  unfolding equiv_hyp_def
+  apply (wpsimp wp: equiv_for_lift assms)
+  apply (rule hoare_weaken_pre)
+   apply (wps assms)
+    apply wpsimp+
+  done
+
+lemma switch_local_fpu_owner_states_equiv_for_non_hyp[wp]:
+  "switch_local_fpu_owner vopt \<lbrace>states_equiv_for_non_fpu P Q R S st\<rbrace>"
+  unfolding states_equiv_for_non_fpu_def
+  by (wpsimp wp: equiv_machine_state_lift equiv_asids_lift equiv_hyp_lift equiv_for_lift dmo_wp)
+
+lemma valid_cur_fpu_hw_fpu_of:
+  "valid_cur_fpu s \<Longrightarrow>
+   hw_fpu_of s t = (if current_fpu s = Some t
+                    then fpu_of (tcb_cur_fpu_of s t) (tcb_fpu_of s t) (machine_fpu s)
+                    else None)"
+  supply if_split[split del]
+  apply (subst fpu_of_def)
+  apply (clarsimp simp: is_arch_cur_fpu_def hw_fpu_def)
+  apply (case_tac "current_fpu s = Some t"; clarsimp)
+  apply (frule (1) current_fpu_owner_Some_tcb_at)
+  apply (clarsimp simp: tcb_at_def get_tcb_def split: option.splits kernel_object.splits)
+  apply (clarsimp simp: valid_cur_fpu_def)
+  apply (erule_tac x=t in allE)
+  apply (clarsimp simp: is_tcb_cur_fpu_def obj_at_def)
+  done
+
+lemma set_arm_current_fpu_owner_current_fpu[wp]:
+  "\<lbrace>\<lambda>s. P (new_owner)\<rbrace>
+   set_arm_current_fpu_owner new_owner
+   \<lbrace>\<lambda>_ s. P (current_fpu s)\<rbrace>"
+  unfolding set_arm_current_fpu_owner_def
+  apply wpsimp
+  apply auto
+  done
+
+crunch switch_local_fpu_owner
+  for valid_cur_fpu[wp]: valid_cur_fpu
+  (wp: hoare_drop_imps)
+
+lemma switch_local_fpu_owner_current_fpu[wp]:
+  "\<lbrace>\<lambda>s. P (new_owner)\<rbrace>
+   switch_local_fpu_owner new_owner
+   \<lbrace>\<lambda>_ s. P (current_fpu s)\<rbrace>"
+  unfolding switch_local_fpu_owner_def
+  by wpsimp
+
+lemma switch_local_fpu_owner_hw_fpu_of:
+  "\<lbrace>\<lambda>s. valid_cur_fpu s \<and> fopt = (if new_owner \<noteq> Some ptr then None
+                                  else if hw_fpu_of s ptr = None then tcb_fpu_of s ptr
+                                  else hw_fpu_of s ptr)\<rbrace>
+   switch_local_fpu_owner new_owner
+   \<lbrace>\<lambda>_ s. fopt = hw_fpu_of s ptr\<rbrace>"
+  apply (rule_tac Q'="\<lambda>_ s. valid_cur_fpu s \<and>
+                            (current_fpu s = Some ptr \<longrightarrow> fopt = fpu_of (tcb_cur_fpu_of s ptr)
+                                                                        (tcb_fpu_of s ptr) (machine_fpu s)) \<and>
+                            (current_fpu s \<noteq> Some ptr \<longrightarrow> fopt = None)"
+               in hoare_strengthen_post[rotated])
+   apply (clarsimp simp: valid_cur_fpu_hw_fpu_of)
+  apply (rule wp_pre)
+   apply (rule hoare_vcg_conj_lift)
+    apply wpsimp
+   apply (rule hoare_vcg_conj_lift)
+    apply (rule hoare_vcg_imp_lift')
+     apply wp
+    apply (wp switch_local_fpu_owner_fpu_of)
+   apply wp
+  apply (clarsimp simp: valid_cur_fpu_hw_fpu_of split: if_splits)
+   apply (simp add: valid_cur_fpu_current_fpu_Some)
+  apply (clarsimp simp: fpu_of_def get_tcb_def split: option.splits bool.splits kernel_object.splits)
+  by (simp add: valid_cur_fpu_defs(1,2,3))
+
+lemma switch_local_fpu_owner_equiv_fpu:
+  "equiv_valid (equiv_fpu P) (equiv_for P kheap) \<top>\<top> valid_cur_fpu (switch_local_fpu_owner new_owner)"
+  apply (clarsimp simp: equiv_fpu_def equiv_valid_def2 equiv_valid_2_def)
+  apply (rename_tac s' t')
+  apply (clarsimp simp: equiv_for_def)
+  apply (erule_tac x=x in allE)+
+  apply clarsimp
+  apply (rule sym)
+  apply (erule use_valid)
+   apply (rule switch_local_fpu_owner_hw_fpu_of)
+  apply (rule conjI, simp)
+  apply (rule sym)
+  apply (erule use_valid)
+   apply (rule switch_local_fpu_owner_hw_fpu_of)
+  apply (rule conjI, simp)
+  apply (case_tac "new_owner \<noteq> Some x")
+   apply clarsimp
+  apply (case_tac "hw_fpu_of s x = None")
+   apply (clarsimp simp: get_tcb_def)
+  apply clarsimp
+  done
+
+lemma switch_local_fpu_owner_states_equiv_valid[wp]:
+  "states_equiv_valid aag L (valid_cur_fpu) (switch_local_fpu_owner new_owner)"
+  apply (rule equiv_valid_conseq)
+    apply (rule equiv_valid_split)
+     apply (rule states_equiv_valid_non_fpu_unobservable[of _ L aag])
+          apply ((wpsimp simp: fpu_restore_def wp: dmo_wp)+)[6]
+    apply (rule equiv_valid_split)
+     apply (rule_tac aag=aag and L=L in switch_local_fpu_owner_equiv_kheap)
+    apply (rule_tac P="L o pasObjectAbs aag" in switch_local_fpu_owner_equiv_fpu)
+   apply (clarsimp simp: states_equiv_for_def states_equiv_for_non_fpu_def comp_def)+
+  done
+
+lemma switch_local_fpu_owner_reads_respects[wp]:
+  "reads_respects aag l (valid_cur_fpu) (switch_local_fpu_owner new_owner)"
+  apply (rule equiv_valid_guard_imp)
+   apply (rule reads_respects_from_labels)
+        apply (rule switch_local_fpu_owner_states_equiv_valid)
+       apply wpsimp+
+  done
+
+lemma arch_thread_set_equiv_but_for_labels[wp]:
+  "\<lbrace>equiv_but_for_labels aag L st and K (pasObjectAbs aag t \<in> L)\<rbrace>
+   arch_thread_set f t
+   \<lbrace>\<lambda>_. equiv_but_for_labels aag L st\<rbrace>"
+  unfolding arch_thread_set_def
+  apply (wpsimp wp: set_object_equiv_but_for_labels)
+  apply (clarsimp simp: get_tcb_def obj_at_def split: option.splits kernel_object.splits)
+  done
+
+lemma modify_current_fpu_equiv_but_for_labels:
+  "\<lbrace>\<lambda>s. equiv_but_for_labels aag L st s \<and>
+        (\<forall>t. current_fpu s = Some t \<longrightarrow> pasObjectAbs aag t \<in> L) \<and>
+        (\<forall>t. new_owner = Some t \<longrightarrow> pasObjectAbs aag t \<in> L)\<rbrace>
+   modify (\<lambda>s. s\<lparr>arch_state := arch_state s\<lparr>arm_current_fpu_owner := new_owner\<rparr>\<rparr>)
+   \<lbrace>\<lambda>_. equiv_but_for_labels aag L st\<rbrace>"
+  apply wp
+  apply (subst equiv_but_for_labels_def)
+  apply (subst states_equiv_for_def)
+  apply (intro conjI; (clarsimp simp: equiv_but_for_labels_def states_equiv_for_def equiv_for_def; fail)?)
+    apply (clarsimp simp: equiv_but_for_labels_def states_equiv_for_def equiv_for_def)
+    apply (clarsimp simp: equiv_asids_def equiv_asid_def)
+   apply (clarsimp simp: equiv_but_for_labels_def states_equiv_for_def equiv_for_def)
+   apply (clarsimp simp: equiv_hyp_def equiv_for_def)
+  apply (prop_tac "equiv_fpu (\<lambda>x. pasObjectAbs aag x \<notin> L) st s")
+   apply (clarsimp simp: equiv_but_for_labels_def states_equiv_for_def equiv_for_def)
+  apply (erule equiv_fpu_trans)
+  apply (clarsimp simp: equiv_fpu_def)
+  apply (clarsimp simp: equiv_for_def)
+  apply (clarsimp simp: is_arch_cur_fpu_def)
+  apply (clarsimp simp: hw_fpu_def)
+  apply auto
+  done
+
+lemma set_arm_current_fpu_owner_equiv_but_for_labels[wp]:
+  "\<lbrace>\<lambda>s. equiv_but_for_labels aag L st s \<and> (\<forall>t. new_owner = Some t \<longrightarrow> pasObjectAbs aag t \<in> L) \<and>
+                                          (\<forall>t. current_fpu s = Some t \<longrightarrow> pasObjectAbs aag t \<in> L)\<rbrace>
+   set_arm_current_fpu_owner new_owner
+   \<lbrace>\<lambda>_. equiv_but_for_labels aag L st\<rbrace>"
+  unfolding set_arm_current_fpu_owner_def
+  by (wpsimp wp_del: modify_wp wp: hoare_vcg_imp_lift' hoare_vcg_all_lift modify_current_fpu_equiv_but_for_labels)
+
+lemma dmo_equiv_but_for_labels_fpu:
+  assumes "\<And>P. f \<lbrace>\<lambda>ms. P (underlying_memory ms)\<rbrace>"
+  assumes "\<And>P. f \<lbrace>\<lambda>ms. P (device_state ms)\<rbrace>"
+  assumes "\<And>P. f \<lbrace>\<lambda>ms. P (irq_state ms)\<rbrace>"
+  assumes "\<And>P. f \<lbrace>\<lambda>ms. P (vcpu_state ms)\<rbrace>"
+  shows "\<lbrace>\<lambda>s. equiv_but_for_labels aag L st s \<and> \<not>cur_fpu_for (\<lambda>x. pasObjectAbs aag x \<notin> L) s\<rbrace>
+         do_machine_op f
+         \<lbrace>\<lambda>_. equiv_but_for_labels aag L st\<rbrace>"
+  unfolding equiv_but_for_labels_def states_equiv_for_def equiv_asids_def cur_fpu_for_def
+  apply wp
+   apply clarsimp
+   apply (rule hoare_vcg_conj_lift, solves "wpsimp wp: equiv_for_lift equiv_hyp_lift assms dmo_wp")+
+   apply (rule hoare_vcg_conj_lift)
+    apply (clarsimp simp: equiv_fpu_def)
+    apply (rule_tac Q'="\<lambda>_ s. (\<forall>x. pasObjectAbs aag x \<notin> L \<longrightarrow> hw_fpu_of st x = None) \<and>
+                              \<not>cur_fpu_for (\<lambda>x. pasObjectAbs aag x \<notin> L) s"
+                 in hoare_strengthen_post)
+     apply (wpsimp wp: equiv_for_lift2 assms dmo_wp simp: cur_fpu_for_def)
+    apply (clarsimp simp: equiv_for_def hw_fpu_def)
+    apply (erule_tac x=x in allE)
+    apply (clarsimp split: if_splits)
+    apply (fastforce simp: cur_fpu_for_def)
+   apply (wpsimp wp: equiv_for_lift equiv_hyp_lift assms dmo_wp)
+  apply clarsimp
+  apply (clarsimp simp: equiv_fpu_def)
+  apply (fastforce simp: equiv_for_def cur_fpu_for_def hw_fpu_def split: if_splits)
+  done
+
+lemma as_user_cur_fpu_for[wp]:
+  "as_user t f \<lbrace>\<lambda>s. P (cur_fpu_for R s)\<rbrace>"
+  apply (wpsimp wp: as_user_wp_thread_set_helper thread_set_wp)
+  apply (auto elim!: rsubst[where P=P]
+               simp: get_tcb_def cur_fpu_for_def arch_tcb_context_get_def arch_tcb_context_set_def)
+  done
+
+lemma dmo_cur_fpu_for[wp]:
+  "do_machine_op f \<lbrace>\<lambda>s. P (cur_fpu_for R s)\<rbrace>"
+  by (wpsimp wp: dmo_wp simp: cur_fpu_for_def)
+
+crunch save_fpu_state
+  for cur_fpu_for[wp]: "\<lambda>s. P (cur_fpu_for R s)"
+
+lemma load_fpu_state_equiv_but_for_labels[wp]:
+  "\<lbrace>\<lambda>s. equiv_but_for_labels aag L st s \<and> \<not>cur_fpu_for (\<lambda>a. pasObjectAbs aag a \<notin> L) s\<rbrace>
+   load_fpu_state t
+   \<lbrace>\<lambda>_. equiv_but_for_labels aag L st\<rbrace>"
+  unfolding load_fpu_state_def
+  by (wpsimp wp: dmo_equiv_but_for_labels_fpu as_user_inv)
+
+lemma switch_local_fpu_owner_equiv_but_for_labels:
+  "\<lbrace>\<lambda>s. equiv_but_for_labels aag L st s \<and> (\<forall>t. cur_fpu_of s t \<longrightarrow> pasObjectAbs aag t \<in> L) \<and>
+                                          (\<forall>t. new_owner = Some t \<longrightarrow> pasObjectAbs aag t \<in> L)\<rbrace>
+   switch_local_fpu_owner new_owner
+   \<lbrace>\<lambda>_. equiv_but_for_labels aag L st\<rbrace>"
+  unfolding switch_local_fpu_owner_def
+  apply (wpsimp wp: hoare_vcg_imp_lift' hoare_vcg_all_lift)
+  apply (prop_tac "equiv_fpu (\<lambda>a. pasObjectAbs aag a \<notin> L) st s")
+   apply (clarsimp simp: equiv_but_for_labels_def states_equiv_for_def)
+  apply (clarsimp simp: cur_fpu_for_def is_arch_cur_fpu_def)
+  done
+
+lemma fpu_release_reads_respects:
+  "reads_respects aag l valid_cur_fpu (fpu_release t)"
+  unfolding fpu_release_def
+  apply (rule equiv_valid_guard_imp)
+   apply (subst gets_comp)
+   apply (rule_tac P=valid_cur_fpu and ptr=t in reads_respects_unit_cases)
+     apply (rule equiv_valid_guard_imp)
+      apply wp
+        apply (wpsimp wp: when_ev)
+       prefer 2
+       apply wpsimp
+      apply (wpsimp wp: gets_ev'')
+      apply (prop_tac "valid_cur_fpu x \<and>  aag_can_read_or_affect aag l t")
+       apply assumption
+      apply (prop_tac "valid_cur_fpu xa \<and>  aag_can_read_or_affect aag l t")
+       apply assumption
+      apply (prop_tac "equiv_fpu (aag_can_read_or_affect aag l) x xa \<and>
+                       equiv_for (aag_can_read_or_affect aag l) kheap x xa ")
+       apply (clarsimp simp: reads_equiv_def2 affects_equiv_def2
+                             states_equiv_for_def equiv_for_disj equiv_fpu_def)
+      apply clarsimp
+      apply (clarsimp simp: valid_cur_fpu_def equiv_for_def is_tcb_cur_fpu_def obj_at_def)
+      apply fastforce
+     apply clarsimp
+    apply wpsimp+
+      apply (wp switch_local_fpu_owner_equiv_but_for_labels)
+     apply (clarsimp split del: if_split cong: if_cong conj_cong)
+     apply wp
+    apply clarsimp
+   apply wpsimp+
+  done
+
+lemma prepare_thread_delete_reads_respects:
+  assumes domains_distinct[wp]: "pas_domains_distinct aag"
+  shows "reads_respects aag l (pas_refined aag and valid_arch_state and valid_cur_fpu and K (is_subject aag thread))
+                              (prepare_thread_delete thread)"
+  unfolding prepare_thread_delete_def
+  apply (wpsimp wp: fpu_release_reads_respects dissociate_vcpu_tcb_reads_respects hoare_vcg_imp_lift'
+         | rule arch_thread_get_wp)+
+  apply (subgoal_tac "is_subject aag x")
+   apply fastforce
+  apply (erule associated_vcpu_is_subject)
+    apply (simp add: get_tcb_ko_at)
+   apply simp
+  apply simp
+  done
+
 lemma prepare_thread_delete_reads_respects_f[Finalise_IF_assms]:
-  "reads_respects_f aag l \<top> (prepare_thread_delete thread)"
-  unfolding prepare_thread_delete_def by wp
+  assumes domains_distinct[wp]: "pas_domains_distinct aag"
+  shows "reads_respects_f aag l (silc_inv aag st and pas_refined aag and valid_arch_state
+                                                 and valid_cur_fpu and K (is_subject aag thread))
+                                (prepare_thread_delete thread)"
+  apply (rule equiv_valid_guard_imp)
+   apply (wpsimp wp: reads_respects_f[OF prepare_thread_delete_reads_respects, where st=st])+
+  done
+
+lemma vcpu_finalise_reads_respects:
+  assumes domains_distinct[wp]: "pas_domains_distinct aag"
+  shows "reads_respects aag l (pas_refined aag and valid_arch_state and K (is_subject aag vr)) (vcpu_finalise vr)"
+  unfolding vcpu_finalise_def
+  apply (rule gen_asm_ev)
+  apply (wpsimp wp: dissociate_vcpu_tcb_reads_respects get_vcpu_wp)
+  apply (fastforce dest: associated_tcb_is_subject)
+  done
 
 lemma arch_finalise_cap_reads_respects[Finalise_IF_assms]:
+  assumes domains_distinct[wp]: "pas_domains_distinct aag"
+  shows
   "reads_respects aag l (pas_refined aag and invs and cte_wp_at ((=) (ArchObjectCap cap)) slot
                                          and K (pas_cap_cur_auth aag (ArchObjectCap cap)))
                         (arch_finalise_cap cap final)"
@@ -257,15 +974,27 @@ lemma arch_finalise_cap_reads_respects[Finalise_IF_assms]:
      apply simp
      apply (simp split: bool.splits)
      apply (intro impI conjI)
-  by (wp delete_asid_pool_reads_respects unmap_page_reads_respects unmap_page_table_reads_respects
-         delete_asid_reads_respects find_vspace_for_asid_reads_respects
-      | simp add: invs_psp_aligned invs_vspace_objs invs_valid_objs valid_cap_def
-                  valid_arch_state_asid_table invs_arch_state wellformed_mapdata_def
-           split: option.splits bool.splits
-      | intro impI conjI allI
-      | elim conjE
-      | drule cte_wp_valid_cap
-      | fastforce dest: aag_can_read_own_asids aag_cap_auth_subject)+
+         apply (wp delete_asid_pool_reads_respects unmap_page_reads_respects unmap_page_table_reads_respects
+                   delete_asid_reads_respects find_vspace_for_asid_reads_respects vcpu_finalise_reads_respects
+                | simp add: invs_psp_aligned invs_vspace_objs invs_valid_objs valid_cap_def
+                            valid_arch_state_asid_table invs_arch_state wellformed_mapdata_def
+                     split: option.splits bool.splits pt_type.splits
+                | intro impI conjI allI
+                | elim conjE
+                | drule cte_wp_valid_cap
+                | fastforce dest: aag_can_read_own_asids aag_cap_auth_subject)+
+     apply (clarsimp simp: aag_cap_auth_def cap_auth_conferred_def arch_cap_auth_conferred_def)
+     apply (drule (1) pas_refined_Control, clarsimp)
+    apply (wp delete_asid_pool_reads_respects unmap_page_reads_respects unmap_page_table_reads_respects
+              delete_asid_reads_respects find_vspace_for_asid_reads_respects vcpu_finalise_reads_respects
+           | simp add: invs_psp_aligned invs_vspace_objs invs_valid_objs valid_cap_def
+                       valid_arch_state_asid_table invs_arch_state wellformed_mapdata_def
+                split: option.splits bool.splits pt_type.splits
+           | intro impI conjI allI
+           | elim conjE
+           | drule cte_wp_valid_cap
+           | fastforce dest: aag_can_read_own_asids aag_cap_auth_subject)+
+  done
 
 (*NOTE: Required to dance around the issue of the base potentially
         being zero and thus we can't conclude it is in the current subject.*)
@@ -277,15 +1006,16 @@ lemma requiv_arm_asid_table_asid_high_bits_of_asid_eq':
    apply (case_tac "b = 0")
     apply (subgoal_tac "is_subject_asid aag 1")
      apply ((fastforce intro: requiv_arm_asid_table_asid_high_bits_of_asid_eq
-                              aag_cap_auth_ASIDPoolCap_asid)+)[2]
+                              aag_cap_auth_ASIDPoolCap_asid
+                    simp del: asid_high_bits_of_0)+)[2]
    apply (auto intro: requiv_arm_asid_table_asid_high_bits_of_asid_eq
                       aag_cap_auth_ASIDPoolCap_asid)[1]
   apply (simp add: asid_high_bits_of_def asid_low_bits_def)
   done
 
 lemma pt_cap_aligned:
-  "\<lbrakk> caps_of_state s p = Some (ArchObjectCap (PageTableCap word x)); valid_caps (caps_of_state s) s \<rbrakk>
-     \<Longrightarrow> is_aligned word pt_bits"
+  "\<lbrakk> caps_of_state s p = Some (ArchObjectCap (PageTableCap word pt_t x)); valid_caps (caps_of_state s) s \<rbrakk>
+     \<Longrightarrow> is_aligned word (pt_bits pt_t)"
   by (auto simp: obj_ref_of_def pt_bits_def pageBits_def
           dest!: cap_aligned_valid[OF valid_capsD, unfolded cap_aligned_def, THEN conjunct1])
 
@@ -321,7 +1051,37 @@ lemma delete_asid_globals_equiv:
    delete_asid asid pt
    \<lbrace>\<lambda>_. globals_equiv st\<rbrace>"
   unfolding delete_asid_def
-  by (wpsimp wp: set_vm_root_globals_equiv set_asid_pool_globals_equiv simp: hwASIDFlush_def)
+  by (wpsimp wp: set_vm_root_globals_equiv set_asid_pool_globals_equiv hoare_drop_imps)
+
+lemma vcpu_finalise_globals_equiv[wp]:
+  "\<lbrace>globals_equiv s and invs\<rbrace>
+   vcpu_finalise vr
+   \<lbrace>\<lambda>_. globals_equiv s\<rbrace>"
+  unfolding vcpu_finalise_def
+  apply (wpsimp wp: dissociate_vcpu_tcb_globals_equiv get_vcpu_wp)
+  apply (rule conjI, fastforce)
+  (* FIXME AARCH64 IF: boilerplate *)
+  apply (rename_tac s' vcpu tcb)
+  apply clarsimp
+  apply (prop_tac "(idle_thread s', HypTCBRef) \<in> state_hyp_refs_of s' vr")
+   apply (clarsimp simp: state_hyp_refs_of_def opt_map_def split: option.splits)
+  apply (drule sym_refsD)
+   apply (erule invs_hyp_sym_refs)
+  apply (clarsimp simp: obj_at_vcpu_hyp_live_of_s[symmetric] is_vcpu_def
+                     state_hyp_refs_of_def obj_at_def hyp_live_def hyp_refs_of_def
+                     tcb_vcpu_refs_def refs_of_ao_def arch_live_def vcpu_tcb_refs_def
+              split: option.splits kernel_object.splits arch_kernel_obj.splits)
+  apply (frule invs_valid_idle)
+  apply (clarsimp simp: valid_idle_def pred_tcb_at_def)
+  apply (frule invs_iflive)
+  apply (frule invs_valid_global_refs)
+  apply (frule invs_valid_objs)
+  apply (drule (1) idle_no_ex_cap)
+  apply (erule swap, erule if_live_then_nonz_capD)
+   apply simp
+  apply clarsimp
+  apply (clarsimp simp: live_def hyp_live_def)
+  done
 
 lemma arch_finalise_cap_globals_equiv[Finalise_IF_assms]:
   "\<lbrace>globals_equiv st and invs and valid_arch_cap cap\<rbrace>
@@ -330,13 +1090,123 @@ lemma arch_finalise_cap_globals_equiv[Finalise_IF_assms]:
   apply (induct cap; simp add: arch_finalise_cap_def)
   by (wp delete_asid_pool_globals_equiv case_option_wp unmap_page_globals_equiv
          unmap_page_table_globals_equiv delete_asid_globals_equiv
-      | wpc | clarsimp simp: valid_arch_cap_def wellformed_mapdata_def)+
+      | wpc | fastforce simp: valid_arch_cap_def wellformed_mapdata_def)+
+
+lemma arch_thread_set_fpu_globals_equiv[wp]:
+  "\<lbrace>globals_equiv s and valid_arch_state\<rbrace>
+   arch_thread_set (tcb_cur_fpu_update f) t
+   \<lbrace>\<lambda>_. globals_equiv s\<rbrace>"
+  unfolding arch_thread_set_is_thread_set
+  by (wpsimp wp: thread_set_globals_equiv simp: arch_tcb_context_get_def)
+
+lemma globals_equiv_fpu_owner_update[simp]:
+  "globals_equiv st (s\<lparr>arch_state := arch_state s\<lparr>arm_current_fpu_owner := cf\<rparr>\<rparr>) = globals_equiv st s"
+  by (auto simp: globals_equiv_def)
+
+lemma set_arm_current_fpu_owner_globals_equiv:
+  "\<lbrace>globals_equiv st and valid_arch_state\<rbrace>
+   set_arm_current_fpu_owner new_owner
+   \<lbrace>\<lambda>_. globals_equiv st\<rbrace>"
+  unfolding set_arm_current_fpu_owner_def
+  by (wpsimp wp: hoare_drop_imps hoare_vcg_all_lift)+
+
+lemma load_fpu_state_globals_equiv:
+  "\<lbrace>globals_equiv st and valid_arch_state and (\<lambda>s. t \<noteq> idle_thread s)\<rbrace>
+   load_fpu_state t
+   \<lbrace>\<lambda>_. globals_equiv st\<rbrace>"
+  unfolding load_fpu_state_def
+  by (wpsimp wp: dmo_globals_equiv)
+
+lemma save_fpu_state_globals_equiv:
+  "\<lbrace>globals_equiv st and valid_arch_state and (\<lambda>s. t \<noteq> idle_thread s)\<rbrace>
+   save_fpu_state t
+   \<lbrace>\<lambda>_. globals_equiv st\<rbrace>"
+  unfolding save_fpu_state_def
+  by (wpsimp wp: dmo_globals_equiv)
+
+crunch load_fpu_state, save_fpu_state
+  for valid_arch_state[wp]: valid_arch_state
+
+(* FIXME AARCH64 IF: move *)
+lemma switch_local_fpu_owner_Some_globals_equiv:
+  "\<lbrace>globals_equiv st and invs and (\<lambda>s. t \<noteq> idle_thread s)\<rbrace>
+   switch_local_fpu_owner (Some t)
+   \<lbrace>\<lambda>_. globals_equiv st\<rbrace>"
+  unfolding switch_local_fpu_owner_def
+  apply (wpsimp wp: set_arm_current_fpu_owner_globals_equiv dmo_globals_equiv
+                    load_fpu_state_globals_equiv save_fpu_state_globals_equiv
+                    hoare_vcg_all_lift hoare_vcg_imp_lift')
+  apply (fastforce simp: invs_def valid_state_def valid_pspace_def valid_cur_fpu_def
+                         is_tcb_cur_fpu_def live_def arch_tcb_live_def
+                   dest: idle_no_ex_cap if_live_then_nonz_capD)
+  done
+
+lemma switch_local_fpu_owner_None_globals_equiv:
+  "\<lbrace>globals_equiv st and invs\<rbrace>
+   switch_local_fpu_owner None
+   \<lbrace>\<lambda>_. globals_equiv st\<rbrace>"
+  unfolding switch_local_fpu_owner_def
+  apply (wpsimp wp: set_arm_current_fpu_owner_globals_equiv dmo_globals_equiv
+                    load_fpu_state_globals_equiv save_fpu_state_globals_equiv
+                    hoare_vcg_all_lift hoare_vcg_imp_lift')
+  apply (fastforce simp: invs_def valid_state_def valid_pspace_def valid_cur_fpu_def
+                          is_tcb_cur_fpu_def live_def arch_tcb_live_def
+                    dest: idle_no_ex_cap if_live_then_nonz_capD)
+  done
+
+declare dissociate_vcpu_tcb_globals_equiv[wp del]
+
+(* FIXME AARCH64 IF: consolidate *)
+lemma dissociate_vcpu_tcb_globals_equiv[wp]:
+  "\<lbrace>globals_equiv s and invs\<rbrace>
+   dissociate_vcpu_tcb vr t
+   \<lbrace>\<lambda>_. globals_equiv s\<rbrace>"
+  unfolding dissociate_vcpu_tcb_def
+  apply (wpsimp wp: as_user_globals_equiv simp: arch_tcb_context_get_def as_user_bind)
+       apply (rule_tac Q'="\<lambda>_ s. arm_current_vcpu (arch_state s) = None" in hoare_post_add)
+       apply (clarsimp cong: conj_cong)
+       apply (wpsimp wp: get_vcpu_wp arch_thread_get_wp)+
+  apply (subgoal_tac "(\<forall>tcb. ko_at (TCB tcb) t sa \<longrightarrow>
+                        (\<forall>v. vcpus_of sa vr = Some v \<longrightarrow>
+                             tcb_vcpu (tcb_arch tcb) = Some vr \<and> vcpu_tcb v = Some t \<longrightarrow>
+                             t \<noteq> idle_thread sa))")
+   apply fastforce
+  apply clarsimp
+  (* FIXME AARCH64 IF: boilerplate *)
+  apply (rename_tac s' tcb vcpu)
+  apply (prop_tac "(idle_thread s', HypTCBRef) \<in> state_hyp_refs_of s' vr")
+   apply (clarsimp simp: state_hyp_refs_of_def opt_map_def split: option.splits)
+  apply (drule sym_refsD)
+   apply (erule invs_hyp_sym_refs)
+  apply (clarsimp simp: obj_at_vcpu_hyp_live_of_s[symmetric] is_vcpu_def
+                        state_hyp_refs_of_def obj_at_def hyp_live_def hyp_refs_of_def
+                        tcb_vcpu_refs_def refs_of_ao_def arch_live_def vcpu_tcb_refs_def
+                 split: option.splits kernel_object.splits arch_kernel_obj.splits)
+  apply (frule invs_valid_idle)
+  apply (clarsimp simp: valid_idle_def pred_tcb_at_def)
+  apply (frule invs_iflive)
+  apply (frule invs_valid_global_refs)
+  apply (frule invs_valid_objs)
+  apply (drule (1) idle_no_ex_cap)
+  apply (erule swap, erule if_live_then_nonz_capD)
+   apply simp
+  apply clarsimp
+  apply (clarsimp simp: live_def hyp_live_def)
+  done
+
+lemma fpu_release_globals_equiv:
+  "\<lbrace>globals_equiv st and invs\<rbrace>
+   fpu_release t
+   \<lbrace>\<lambda>_. globals_equiv st\<rbrace>"
+  unfolding fpu_release_def
+  by (wpsimp wp: switch_local_fpu_owner_None_globals_equiv)
+
+lemma prepare_thread_delete_globals_equiv[Finalise_IF_assms, wp]:
+  "\<lbrace>globals_equiv s and invs\<rbrace> prepare_thread_delete t \<lbrace>\<lambda>_. globals_equiv s\<rbrace>"
+  unfolding prepare_thread_delete_def
+  by (wpsimp wp: fpu_release_globals_equiv hoare_drop_imps)
 
 declare arch_get_sanitise_register_info_def[simp]
-
-crunch prepare_thread_delete
-  for globals_equiv[Finalise_IF_assms, wp]: "globals_equiv st"
-  (wp: dxo_wp_weak)
 
 lemma set_bound_notification_globals_equiv[Finalise_IF_assms]:
   "\<lbrace>globals_equiv s and valid_arch_state\<rbrace>
