proof/infoflow/AARCH64/ArchInfoFlow.thy
@@ -10,7 +10,10 @@ imports
   "Lib.EquivValid"
 begin
 
-context Arch begin global_naming AARCH64
+(* Declare here and define in InfoFlow_IF *)
+consts equiv_for :: "('a \<Rightarrow> bool) \<Rightarrow> ('b \<Rightarrow> 'a \<Rightarrow> 'c) \<Rightarrow> 'b \<Rightarrow> 'b \<Rightarrow> bool"
+
+context Arch begin arch_global_naming
 
 section \<open>Arch-specific equivalence properties\<close>
 
@@ -48,14 +51,71 @@ definition non_asid_pool_kheap_update where
          \<longrightarrow> kheap s x = kh x"
 
 
-subsection \<open>Exclusive machine state equivalence\<close>
+subsection \<open>VCPU equivalence\<close>
+
+(* FIXME AARCH64 IF: move *)
+locale_abbrev numlistregs :: "'s state \<Rightarrow> nat" where
+  "numlistregs s \<equiv> arm_gicvcpu_numlistregs (arch_state s)"
+
+(* FIXME AARCH64 IF: move *)
+locale_abbrev current_vcpu :: "'s state \<rightharpoonup> obj_ref \<times> bool" where
+  "current_vcpu s \<equiv> arm_current_vcpu (arch_state s)"
+
+definition hw_vcpu :: "nat \<Rightarrow> bool option \<Rightarrow> vcpu_state \<rightharpoonup> vcpu_state" where
+  "hw_vcpu n cv vcpu \<equiv> case cv of
+     None \<Rightarrow> None
+   | Some enabled \<Rightarrow> Some
+       \<lparr>vcpu_vgic = \<lparr>vgic_hcr = if \<not>enabled then undefined else vgic_hcr (vcpu_vgic vcpu),
+                     vgic_vmcr = vgic_vmcr (vcpu_vgic vcpu),
+                     vgic_apr = vgic_apr (vcpu_vgic vcpu),
+                     vgic_lr = \<lambda>r. if r < n then vgic_lr (vcpu_vgic vcpu) r else undefined\<rparr>,
+        vcpu_regs = \<lambda>r. if \<not>enabled \<and> vcpuRegSavedWhenDisabled r
+                        then undefined
+                        else vcpu_regs vcpu r\<rparr>"
+
+locale_abbrev hw_vcpu_of :: "'s state \<Rightarrow> obj_ref \<rightharpoonup> vcpu_state" where
+  "hw_vcpu_of s p \<equiv> hw_vcpu (numlistregs s) (cur_vcpu_of s p) (vcpu_state (machine_state s))"
+
+lemmas hw_vcpu_of_def = hw_vcpu_def
+
+definition equiv_hyp :: "(obj_ref \<Rightarrow> bool) \<Rightarrow> det_state \<Rightarrow> det_state \<Rightarrow> bool" where
+  "equiv_hyp P s s' \<equiv> equiv_for P (K \<circ> numlistregs) s s' \<and>
+                       equiv_for P cur_vcpu_of s s' \<and>
+                       equiv_for P hw_vcpu_of s s'"
+
+
+subsection \<open>FPU equivalence\<close>
+
+(* FIXME AARCH64 IF: move *)
+locale_abbrev current_fpu :: "'s state \<rightharpoonup> obj_ref" where
+  "current_fpu s \<equiv> arm_current_fpu_owner (arch_state s)"
+
+definition is_arch_cur_fpu_2 :: "obj_ref \<Rightarrow> obj_ref option \<Rightarrow> bool" where
+  "is_arch_cur_fpu_2 ptr fopt \<equiv> fopt = Some ptr"
+
+locale_abbrev is_arch_cur_fpu :: "obj_ref \<Rightarrow> 's state \<Rightarrow> bool" where
+  "is_arch_cur_fpu ptr s \<equiv> is_arch_cur_fpu_2 ptr (arm_current_fpu_owner (arch_state s))"
+
+lemmas is_arch_cur_fpu_def = is_arch_cur_fpu_2_def
+
+definition hw_fpu :: "bool \<Rightarrow> fpu_state \<Rightarrow> fpu_state option" where
+  "hw_fpu cf fpu \<equiv> if cf then Some fpu else None"
+
+locale_abbrev hw_fpu_of :: "'s state \<Rightarrow> 64 word \<rightharpoonup> fpu_state" where
+  "hw_fpu_of s t \<equiv> hw_fpu (is_arch_cur_fpu t s) (fpu_state (machine_state s))"
+
+definition equiv_fpu :: "(obj_ref \<Rightarrow> bool) \<Rightarrow> det_state \<Rightarrow> det_state \<Rightarrow> bool" where
+  "equiv_fpu P s s' \<equiv> equiv_for P hw_fpu_of s s'"
+
 
 subsection \<open>Global (Kernel) VSpace equivalence\<close>
 (* globals_equiv should be maintained by everything except the scheduler, since
    nothing else touches the globals frame *)
 
-definition arch_globals_equiv :: "obj_ref \<Rightarrow> obj_ref \<Rightarrow> kheap \<Rightarrow> kheap \<Rightarrow> arch_state \<Rightarrow>
-                                  arch_state \<Rightarrow> machine_state \<Rightarrow> machine_state \<Rightarrow> bool" where
+definition arch_globals_equiv ::
+  "obj_ref \<Rightarrow> obj_ref \<Rightarrow> kheap \<Rightarrow> kheap \<Rightarrow> arch_state \<Rightarrow>
+   arch_state \<Rightarrow> machine_state \<Rightarrow> machine_state \<Rightarrow> bool"
+  where
   "arch_globals_equiv ct it kh kh' as as' ms ms' \<equiv>
      arm_us_global_vspace as = arm_us_global_vspace as' \<and>
      kh (arm_us_global_vspace as) = kh' (arm_us_global_vspace as)"
@@ -64,10 +124,11 @@ declare arch_globals_equiv_def[simp]
 
 end
 
-requalify_consts
-  AARCH64.equiv_asid
-  AARCH64.equiv_asid'
-  AARCH64.arch_globals_equiv
-  AARCH64.non_asid_pool_kheap_update
+(* FIXME AARCH64 IF: requalify elsewhere *)
+arch_requalify_consts
+  equiv_asid
+  equiv_asid'
+  arch_globals_equiv
+  non_asid_pool_kheap_update
 
 end
